

## *Directional Statistics*

by K. V. Mardia & P. E. Jupp

Wiley, Chichester, 2000.

### **Errata to 1st printing**

- 8<sup>4</sup> Insert ‘of’ after ‘development’.
- 17<sup>3</sup> Replace ‘ $\theta_1 - \alpha, \dots, \theta_1 - \alpha$ ’ by ‘ $\theta_1 - \alpha, \dots, \theta_n - \alpha$ ’.
- 19<sub>1</sub> = (2.3.14) Replace ‘ $\theta$ ’ by ‘ $\theta_i$ ’.
- 20<sub>7</sub> Replace ‘13, 13’ by ‘13, 0’.
- 22<sup>4</sup> = (2.4.10) The right hand side should be

$$-c^3 \frac{1}{n} \sum_{i=1}^n (x_i - \bar{x})^3 + O(c^5)$$

- 22<sup>5</sup> = (2.4.11) The right hand side should be

$$1 - 2c^2 \frac{1}{n} \sum_{i=1}^n (x_i - \bar{x})^2 + \frac{2c^4}{3} \frac{1}{n} \sum_{i=1}^n (x_i - \bar{x})^4 + O(c^6).$$

- 22<sub>5</sub> Replace ‘ $m_2 = 0.383 + 0.491i$ ’ by ‘ $m_2 = 0.383 - 0.030i$ ’.
- 22<sub>3</sub> Replace ‘ $\hat{s} = 0.322$ ’ by ‘ $\hat{s} = -0.196$ ’.
- 32<sub>3</sub> = (3.5.3) Replace  $\frac{\partial \psi}{\partial \boldsymbol{\theta}}$  by  $\frac{\partial \psi}{\partial \boldsymbol{\theta}^T}$ .
- 38<sup>4</sup> = (3.5.22) Replace ‘ $\kappa^{-1/2}(\theta - \mu)$ ’ by ‘ $\kappa^{1/2}(\theta - \mu)$ ’.
- 46<sup>14</sup> = (3.5.48) Replace the term ‘ $\phi(\theta; \mathbf{0}, \boldsymbol{\Sigma})$ ’ in the denominator by ‘ $\phi(\boldsymbol{\mu}; \mathbf{0}, \boldsymbol{\Sigma})$ ’.
- 47<sub>1</sub> = (3.5.55) Replace  $e^{2\pi i x}$  by  $e^{ix}$ .
- 51<sup>13</sup> Replace  $e^{-a|t| - it\mu}$  by  $e^{-a|t| + it\mu}$ .
- 51<sub>6</sub> = (3.5.70) Replace ‘ $\phi_p = \rho^{|p|}$ ,  $\alpha_p = \rho^{|p|} \cos \mu$ ,  $\beta_p = \rho^{|p|} \sin \mu$ ’  
by ‘ $\phi_p = \rho^{|p|} e^{ip\mu}$ ,  $\alpha_p = \rho^{|p|} \cos p\mu$ ,  $\beta_p = \rho^{|p|} \sin p\mu$ ’.
- 58<sup>5-6</sup> Replace ‘square-summable’ by ‘square-integrable’.
- 58<sup>13</sup> Replace ‘square-summable’ by ‘square-integrable’.

67<sub>3</sub> = (4.4.12) Replace ‘ $\simeq$ ’ by ‘ $=$ ’.

80<sub>1</sub> Replace ‘ $n\text{var}\bar{R}$ ’ by ‘ $n\text{var}(\bar{R})$ ’.

89<sub>9</sub> Insert ‘(up to addition of a constant)’ after ‘is’.

89<sub>8</sub> = (5.4.3) The right hand side should be

$$\frac{n}{2} \log(1 - \|\boldsymbol{\mu}\|^2) - \sum_{i=1}^n \log(1 - \boldsymbol{\mu}^T \mathbf{x}_i).$$

90<sup>10</sup> Replace

$$\hat{\rho}^2 = \frac{1 - \sqrt{1 - \|\hat{\boldsymbol{\mu}}\|^2}}{1 + \sqrt{1 - \|\hat{\boldsymbol{\mu}}\|^2}} \quad \text{by} \quad \hat{\rho} = \frac{1 - \sqrt{1 - \|\hat{\boldsymbol{\mu}}\|^2}}{\|\hat{\boldsymbol{\mu}}\|}.$$

91<sub>6-4</sub> The model with density (5.5.4) is not a special case of (5.5.2).  
It is symmetrical about 0 and, for large enough values of  $\mu$ ,  
it has modes at  $\pm\mu$ .

95<sup>7</sup> Replace ‘ $O(n^{-1/2})$ ’ by ‘ $O(n^{-1})$ ’.

95<sup>13</sup> Replace ‘ $O(n^{-1})$ ’ by ‘ $O(n^{-2})$ ’.

Replace ‘1999’ by ‘2001’.

95<sub>4</sub> = (6.3.8) This should be

$$w = 2n \{ \hat{\kappa} \bar{R} - \log I_0(\hat{\kappa}) \} = 2n \{ \hat{\kappa} A(\hat{\kappa}) - \log I_0(\hat{\kappa}) \}.$$

95<sub>2</sub> The right hand side should be

$$2n \{ A(\hat{\kappa}) + \hat{\kappa} A'(\hat{\kappa}) - A(\hat{\kappa}) \}.$$

108<sub>12</sub> Delete ‘the’.

113<sup>5</sup> Replace

$$\sum_{i=1}^n \sum_{j=1}^n \quad \text{by} \quad \sum_{i=1}^n \sum_{j \neq i}^n.$$

117<sup>2</sup> = (6.4.3) The right hand side should be

$$\sum_{j=1}^k p_j S_j.$$

117<sup>4</sup> = (6.4.4) The right hand side should be

$$\frac{1}{n} \sum_{j=1}^k (S_j - \bar{S})^2 p_j$$

123<sub>10</sub> = (7.2.23) The right hand side should be  $2\kappa(n - R) + 2\kappa(R - C)$ .

139<sup>11-23</sup> This subsection should be moved to the end of subsection 7.4.2 on page 141 (between lines 141<sub>11</sub> and 141<sub>10</sub>), replacing ‘**ANOVA Based on a**’ (in line 139<sup>11</sup>) by ‘**A**’, replacing ‘asymptotic large-sample’ (in line 139<sub>8</sub>) by ‘high-concentration asymptotic’, renumbering equations as follows:

$$\begin{aligned} (7.4.20) &\mapsto (7.4.17) & (7.4.21) &\mapsto (7.4.18) \\ (7.4.22) &\mapsto (7.4.19) & (7.4.23) &\mapsto (7.4.20) \\ (7.4.24) &\mapsto (7.4.21) & (7.4.25) &\mapsto (7.4.22) \\ (7.4.17) &\mapsto (7.4.23) & (7.4.18) &\mapsto (7.4.24) \\ (7.4.19) &\mapsto (7.4.25) \end{aligned}$$

and replacing equation references as follows:

$$\begin{aligned} 139_8 & \quad (7.4.17) \mapsto (7.4.23) \\ 141_{19} & \quad (7.4.23) \mapsto (7.4.20) \\ 141_{17} & \quad (7.4.23) \mapsto (7.4.20). \end{aligned}$$

138<sub>4</sub> This should be

$$\sum_{i=1}^n \|\mathbf{x}_i - \bar{\mathbf{x}}\|^2 = n(1 - \bar{R}^2).$$

139<sub>9</sub> = (7.4.19) The first equation should be

$$\bar{d}_i = \frac{1}{n_i} \sum_{j=1}^{n_i} d_{ij}.$$

140<sub>12</sub> = (7.4.24) The first term on the right hand side should be

$$\sum_{i=1}^q w_i g_2 (\bar{R}_i)^2.$$

142<sup>14</sup> Delete ‘is’ after ‘Thus’.

140<sub>1</sub> = (7.5.3) This equation should be

$$S = \frac{s_c^2}{nv_c(\hat{\kappa})} + \frac{s_s^2}{nv_s(\hat{\kappa})},$$

143<sup>2</sup> Replace ‘ $-nA(\hat{\kappa})$ ’ by ‘ $-nI_2(\hat{\kappa})/I_0(\hat{\kappa})$ ’.

143<sup>4-6</sup> These equations should be

$$\begin{aligned} v_c(\kappa) &= \frac{I_0(\kappa)^2 + I_0(\kappa)I_4(\kappa) - 2I_2(\kappa)^2}{2I_0(\kappa)^2} \\ &\quad - \frac{(I_0(\kappa)I_3(\kappa) + I_0(\kappa)I_1(\kappa) - 2I_1(\kappa)I_2(\kappa))^2}{2I_0(\kappa)^2(I_0(\kappa)^2 + I_0(\kappa)I_2(\kappa) - 2I_1(\kappa)^2)} \\ v_s(\kappa) &= \frac{(I_0(\kappa) - I_4(\kappa))(I_0(\kappa) - I_2(\kappa)) - (I_1(\kappa) - I_3(\kappa))^2}{2I_0(\kappa)(I_0(\kappa) - I_2(\kappa))}, \end{aligned}$$

143<sup>7</sup> Replace ‘approximations to their variances’ by ‘their conditional variances’.

151<sub>10</sub> Insert ‘Assume that there are no ties.’ before ‘Let  $s_i$  be’.

151<sub>7-4</sub> Replace these lines by

$$\begin{aligned} d_1 &= \frac{1}{n_2}, \dots, d_{s_1} = \frac{s_1}{n_2}, & d_{s_1+1} &= \frac{s_1+1}{n_2} - \frac{1}{n_1}, \dots, \\ d_{s_2} &= \frac{s_2}{n_2} - \frac{1}{n_1}, & d_{s_2+1} &= \frac{s_2}{n_2} - \frac{2}{n_1}, \dots, & d_n &= \frac{n_2}{n_2} - \frac{n_1}{n_1}. \end{aligned}$$

Hence, from (8.3.7) and some algebraic manipulation we obtain

$$U_{n_1, n_2}^2 = \frac{1}{nn_2} \left\{ \sum_{i=1}^{n_1} \left( r_i - \frac{n}{n_1} i \right)^2 - n_1 \left( \bar{r} - \frac{n(n_1+1)}{2n_1} \right)^2 \right\} + \frac{n+n_1}{12nn_1}. \quad (8.3.8)$$

- 161<sub>15-11</sub> Replace this paragraph by  
‘The projection (9.1.1) distorts the lower hemisphere more than the upper hemisphere. If the data are spread over both hemispheres then it is helpful to project the two hemispheres onto separate discs in the plane, using (9.1.1) on the upper hemisphere and the variant which replaces  $\theta$  by  $\pi - \theta$  on the right hand side of (9.1.1) on the lower hemisphere.’
- 162<sup>1-4</sup> Replace ‘tangent vectors  $\dots \mathbf{x}^T \boldsymbol{\mu} = 0$ ’ by ‘tangent vectors  $\mathbf{z}$  to the sphere at  $\boldsymbol{\mu}$  are wrapped onto the sphere by

$$\mathbf{z} \mapsto \cos(\|\mathbf{z}\|) \boldsymbol{\mu} + \frac{\sin(\|\mathbf{z}\|)}{\|\mathbf{z}\|} \mathbf{z} \quad (9.1.3)$$

where  $\mathbf{z}^T \boldsymbol{\mu} = 0$ ’.

- 164<sub>16-14</sub> The equation array should be

$$\begin{aligned} S(\mathbf{a}) &= \frac{1}{n} \sum_{i=1}^n \|\mathbf{x}_i - \mathbf{a}\|^2 \\ &= 2(1 - \bar{\mathbf{x}}^T \mathbf{a}) \\ &= 2(1 - \bar{R} \bar{\mathbf{x}}_0^T \mathbf{a}). \end{aligned} \quad (9.2.3)$$

- 164<sub>13</sub> Replace ‘middle expression’ by ‘last line’.

- 166<sup>2,4</sup> Replace ‘ $\bar{\mathbf{x}}_0$ ’ by ‘ $\bar{\mathbf{x}}$ ’ (3 times).

- 168<sup>19</sup> Replace

$$\frac{\kappa}{2 \sinh \kappa} \exp \{ \kappa \boldsymbol{\mu}^T \mathbf{x} \} \quad \text{by} \quad \frac{\kappa}{\sinh \kappa} \exp \{ \kappa \boldsymbol{\mu}^T \mathbf{x} \}$$

- 169<sup>5</sup> Replace the integral in the numerator by  $\int_{-1}^1 t e^{\kappa t} (1 - t^2)^{(p-3)/2} dt$ .

- 170<sup>3</sup> = (9.3.12) Replace  $I_{(p-1)/2}(\kappa)$  by  $I_{p/2-1}(\kappa)$ .

- 172<sub>10</sub> Replace ‘ $(1 - \|\mathbf{y}\|^2)^{1/2}$ ’ by ‘proportional to  $(1 - \|\mathbf{y}\|^2)^{-1/2}$ ’.

- 173<sub>12</sub> Replace  $M_p(\boldsymbol{\mu}_2, \kappa)$  by  $M_q(\boldsymbol{\mu}_1, \kappa)$ .

- 185<sup>4</sup> Replace  $\bar{\mathbf{x}}_0 | R$  by  $\bar{\mathbf{x}}_0 | \bar{R}$ .

- 185<sup>5</sup> Replace  $\boldsymbol{\mu}_0$  by  $\boldsymbol{\mu}$ .

185<sup>10</sup> Replace ‘(9.5.8)’ by ‘(9.5.6)’.

185<sup>11</sup> This should be

$$\{(\mathbf{x}_1, \dots, \mathbf{x}_n) : \|\bar{\mathbf{x}}\| = \bar{R}, \bar{\mathbf{x}}^T \boldsymbol{\mu} = \bar{C}\}$$

185<sup>14–15</sup> These lines should be

Integration over  $\{(\mathbf{x}_1, \dots, \mathbf{x}_n) : \bar{\mathbf{x}}^T \boldsymbol{\mu} = \bar{C}\}$  gives the density of  $\bar{C}$  as

$$\tilde{g}(\bar{C}; \boldsymbol{\mu}, \kappa) = c(\kappa)^n \exp\{n\kappa\bar{C}\} \tilde{g}(\bar{C}; \boldsymbol{\mu}, 0),$$

and so the conditional density of  $\bar{R}|\bar{C}$  is

$$\frac{g^*(\bar{R}, \bar{C}; \boldsymbol{\mu}, 0)}{\tilde{g}(\bar{C}; \boldsymbol{\mu}, 0)}, \quad (9.5.11)$$

185<sub>1</sub> = (9.5.13) The right hand side should be

$$c(\kappa)^n c(n\kappa\bar{R})^{-1} f(\bar{R}, \bar{R}_1, \dots, \bar{R}_q; \boldsymbol{\mu}, 0).$$

186<sup>3</sup> = (9.5.14) This should be

$$f(\bar{R}_1, \dots, \bar{R}_q | \bar{R}; \kappa) = \frac{f(\bar{R}, \bar{R}_1, \dots, \bar{R}_q; \boldsymbol{\mu}, 0)}{h_n(n\bar{R})}.$$

186<sub>9</sub> This should be

$$\mathbb{E} \left[ \left( \sum_{i=1}^p X_i^2 \right) \left( \sum_{j=1}^p X_j^2 \right) \right] = 1$$

186<sub>7</sub> This should be

$$\mathbb{E}[X_i^4] = \mathbb{E} \left[ \left( \frac{X_i + X_j}{\sqrt{2}} \right)^4 \right] \quad j \neq i$$

190<sup>17</sup> Delete ‘and  $n - t$ ’.

192<sup>7</sup> Replace ‘ $\text{tr } \mathbf{A}$ ’ by ‘ $\kappa_1$ ’.

193<sub>8</sub> Replace ‘ $\mathbf{a} \neq \mathbf{b}$ ’ by ‘ $\mathbf{a} \neq -\mathbf{b}$ ’.

198<sup>14–15</sup> = (10.3.5) This should be

$$I_\nu(\kappa) = (2\pi\kappa)^{-\frac{1}{2}} e^\kappa \left\{ 1 - \frac{4\nu^2 - 1}{8\kappa} + \frac{(4\nu^2 - 1)(4\nu^2 - 9)}{2(8\kappa)^2} \right\} + O(\kappa^{-3}).$$

203<sub>6</sub> This should be

$$l(\mathbf{A}; \pm \mathbf{x}_1, \dots, \pm \mathbf{x}_n) = n \left\{ \text{tr}(\mathbf{A} \bar{\mathbf{T}}) - \log {}_1F_1 \left( \frac{1}{2}, \frac{p}{2}, \mathbf{A} \right) \right\}.$$

207<sub>10</sub> Replace ' $O(n^{-1/2})$ ' by ' $O(n^{-1})$ '.

207<sub>7</sub> Replace ' $O(n^{-1})$ ' by ' $O(n^{-2})$ '.

Replace '1999' by '2001'.

214<sub>8</sub> = (10.4.26) The equation should be ' $\Pr(\mathbf{x}^T \boldsymbol{\mu} \geq \cos \delta) = 1 - \alpha$ '.

215<sub>2</sub> = (10.4.31) The left hand side should be ' $\sin \delta$ '.

220<sub>13,11</sub> Replace ' $1 - \boldsymbol{\mu}_1^T \boldsymbol{\mu}_2$ ' by ' $1 - \bar{\mathbf{x}}_{01}^T \bar{\mathbf{x}}_{02}$ '.

220<sub>8</sub> Replace ' $\mathbf{x}_i^T \boldsymbol{\mu}_i$ ' by ' $\bar{\mathbf{x}}_{0i}^T \boldsymbol{\mu}_i$ '.

225<sub>10</sub> The left hand side should be

$$\sum_{i=1}^n \|\mathbf{x}_i - \bar{\mathbf{x}}\|^2.$$

225<sub>1</sub> = (10.6.19) This should be

$$\frac{(\sum_{i=1}^q n_i \bar{R}_i^2 - n \bar{R}^2)/(q-1)(p-1)}{(n - \sum_{i=1}^q n_i \bar{R}_i^2)/(q-1)(p-1)}.$$

226<sub>10</sub> = (10.6.21) Replace

$$\nu \log \left( \frac{n \sum_{i=1}^q R_i}{\nu} \right) \quad \text{by} \quad \nu \log \left( \frac{n - \sum_{i=1}^q R_i}{\nu} \right).$$

226<sub>8</sub> Replace ' $\nu_i = 2(n_i - 1), \nu = 2(n - q)$ ' by

$$' \nu_i = (p-1)(n_i - 1), \nu = (p-1)(n - q) '.$$

232<sub>3</sub> Replace

$$\frac{p^2 + 6p + 20}{12(p+4)} \quad \text{by} \quad \frac{2p^2 + 3p + 4}{6(p+4)}.$$

232<sub>2</sub> Replace

$$\frac{-(p^2 + 3p + 8)}{3(p+4)(p^2 + p + 2)} \quad \text{by} \quad \frac{-(4p^2 + 3p - 4)}{3(p+4)(p^2 + p + 2)}.$$

232<sub>1</sub> Replace

$$\frac{p^2 - 4}{3(p+4)(p^2+p+2)(p^2+p+6)}$$

by

$$-\frac{4(p^2 - 4)}{3(p+4)(p^2+p+2)(p^2+p+6)}.$$

233<sup>3</sup> Replace ‘ $O(n^{-3/2})$ ’ by ‘ $O(n^{-2})$ ’.

Replace ‘1999’ by ‘2001’.

235<sup>11-12</sup> (10.7.15) and (10.7.16) should be

$$w_b \simeq \frac{n(p^2 - 1) \{ \text{tr}(\bar{\mathbf{T}}^2) - \bar{t}_1^2 - (1 - \bar{t}_1)^2/(p-1) \}}{2(1 - 2\bar{t}_1 + \hat{c}_{11})} \quad (10.7.15)$$

$$w_g \simeq \frac{n(p^2 - 1) \{ \text{tr}(\bar{\mathbf{T}}^2) - \bar{t}_p^2 - (1 - \bar{t}_p)^2/(p-1) \}}{2(1 - 2\bar{t}_p + \hat{c}_{pp})}, \quad (10.7.16)$$

235<sup>14</sup> This line should be

$$\hat{c}_{11} = \frac{1}{n} \sum_{i=1}^n (\mathbf{x}_i^T \mathbf{t}_1)^4 \quad \hat{c}_{pp} = \frac{1}{n} \sum_{i=1}^n (\mathbf{x}_i^T \mathbf{t}_p)^4.$$

235<sub>9-8</sub> (10.7.17) and (10.7.18) should be

$$\frac{n(p^2 - 1) \{ \text{tr}(\bar{\mathbf{T}}^2) - \bar{t}_1^2 - (1 - \bar{t}_1)^2/(p-1) \}}{2(1 - 2\bar{t}_1 + \hat{c}_{11})} \stackrel{\cdot}{\sim} \chi_{(p+1)(p-2)/2}^2 \quad (10.7.17)$$

$$\frac{n(p^2 - 1) \{ \text{tr}(\bar{\mathbf{T}}^2) - \bar{t}_p^2 - (1 - \bar{t}_p)^2/(p-1) \}}{2(1 - 2\bar{t}_p + \hat{c}_{pp})} \stackrel{\cdot}{\sim} \chi_{(p+1)(p-2)/2}^2, \quad (10.7.18)$$

239<sub>13</sub> The right hand side should be

$$\frac{1}{n} \sum_{i=1}^q \sum_{j=1}^{n_i} (\mathbf{x}_{ij}^T \mathbf{t}_p)^4.$$

239<sub>6</sub> = (10.7.40) The right hand side should be

$$\frac{1}{n} \sum_{i=1}^q \sum_{j=1}^{n_i} (\mathbf{x}_{ij}^T \mathbf{t}_1)^4.$$



- 239<sub>4</sub> Replace ‘(10.7.40)’ by ‘(10.7.39)’.
- 247<sub>1</sub> = (11.2.4) Replace ‘ $\sin^4(\pi n)$ ’ in the lower line by ‘ $\sin^4(\pi/n)$ ’.
- 248<sup>3</sup> Replace ‘ $U_n = 0.398$ ’ by ‘ $U_n = 6.73$ ’.
- 248<sup>4</sup> Replace ‘10%’ by ‘5%’.
- Replace ‘4.59 and 4.6’ by ‘5.7 and 5.8’.
- 248<sup>5</sup> Replace ‘accepted’ by ‘rejected’.
- 249<sup>7</sup> Replace ‘ $2(r_{cc}r_{ss} - r_{cs}r_{sc})r_1r_2$ ’ by ‘ $2(r_{cc}r_{ss} + r_{cs}r_{sc})r_1r_2$ ’.
- 249<sub>8</sub> Replace ‘ $r_{cc}^2 = 0.974$ ,  $r_{cs}^2 = 0.213$ ,  $r_{sc}^2 = 0.152$ ,  $r_{ss}^2 = 0.933$ ’ by  
‘ $r_{cc} = 0.993$ ,  $r_{cs} = 0.646$ ,  $r_{sc} = 0.719$ ,  $r_{ss} = 0.960$ ’.
- 249<sub>7</sub> Replace ‘0.714’ by ‘0.713’.
- Replace ‘ $r^2 = 6.64$ ’ by ‘ $r^2 = 1.87$ ’.
- 249<sub>5</sub> Replace ‘ $nr^2 = 66.4$ ’ by ‘ $nr^2 = 18.7$ ’.
- 254<sub>10</sub> This should be

$$\mathbf{S}^* = \frac{1}{n} \sum_{i=1}^n \begin{pmatrix} \mathbf{x}_i \mathbf{x}_i^T & \mathbf{x}_i \mathbf{y}_i^T \\ \mathbf{y}_i \mathbf{x}_i^T & \mathbf{y}_i \mathbf{y}_i^T \end{pmatrix} = \begin{pmatrix} \mathbf{S}_{11}^* & \mathbf{S}_{21}^* \\ \mathbf{S}_{21}^* & \mathbf{S}_{22}^* \end{pmatrix},$$

- 262<sup>8</sup> Replace ‘ $\mathbf{A}^T \mathbf{A} = \mathbf{I}_2$  and  $\mathbf{A} \mathbf{b} = \mathbf{0}$ ’ by  
‘ $\mathbf{A}^T \mathbf{A} = (1 - \|\mathbf{b}\|^2) \mathbf{I}_2$ ,  $\mathbf{A}^T \mathbf{b} = \mathbf{0}$  and  $\|\mathbf{b}\| \leq 1$ ’.
- 264<sub>16</sub> Replace ‘is a’ by ‘is an’.
- 269<sub>4</sub> = (12.3.3) This should be  $F(x) = 1 - \exp(-\hat{\kappa}x)$ .
- 269<sub>2</sub> This should be

$$\hat{\kappa} = \frac{n-1}{\sum_{i=1}^n (1 - \cos \theta'_i)} = \frac{n-1}{n(1 - \bar{R})}$$

- 270<sup>8</sup> Replace ‘ $\phi_i'' \sqrt{\theta_i''}$ ’ by ‘ $\phi_i'' \sqrt{\sin \theta_i''}$ ’.
- 271<sup>2</sup> Replace ‘0.530’ by ‘0.389’.
- 271<sup>6</sup> Replace ‘0.953’ by ‘0.885’.
- 271<sup>9</sup> Replace ‘0.250’ by ‘0.490’.
- 279<sup>5</sup> The left hand side should be just  $\hat{f}_T$ .

287<sub>8</sub> Replace ' $O(n^{-1/2})$ ' by ' $O(n^{-1})$ '.

287<sub>4</sub> Replace ' $O(n^{-1})$ ' by ' $O(n^{-2})$ '.

Replace '1999' by '2001'.

289<sub>5</sub> Replace 'Fisher matrix' by 'matrix Fisher'.

293<sub>10</sub> Replace 'in in' by 'in'.

294<sub>11</sub> Replace ' $O(n^{-1/2})$ ' by ' $O(n^{-1})$ '.

294<sub>5</sub> Replace

$$\frac{p^2(p^2 + p - 2) + 2r(p - r)(p^2 + 4p - 20)}{12r(p - r)(p - 2)(p - 1)(p + 4)(p + 2)}$$

by

$$\frac{2p^2(p - 1)(p + 2) - r(p - r)(5p^2 + 2p + 8)}{6r(p - r)(p - 2)(p + 4)}.$$

294<sub>4</sub> Replace

$$- \left[ \frac{p^2(p^2 + p - 2) - r(p - r)(p^2 - 2p + 16)}{3r(p - r)(p^2 + p + 2)(p - 2)(p + 4)} \right]$$

by

$$- \left[ \frac{4p^2(p - 1)(p + 2) - r(p - r)(13p^2 + 10p - 8)}{3r(p - r)(p^2 + p + 2)(p - 2)(p + 4)} \right].$$

294<sub>3</sub> Replace

$$\frac{(p - 2r)^2(p - 1)(p + 2)}{3r(p - r)(p - 2)(p + 4)(p^2 + p + 2)(p^2 + p + 6)}$$

by

$$\frac{4(p - 2r)^2(p - 1)(p + 2)}{3r(p - r)(p - 2)(p + 4)(p^2 + p + 2)(p^2 + p + 6)}.$$

294<sub>1</sub> Replace ' $O(n^{-1})$ ' by ' $O(n^{-2})$ '.

Replace '1999' by '2001'.

300<sub>8</sub> Delete 'If  $\mathbf{H}$  is invertible'.

- 306<sub>5</sub> Delete ‘a’ before ‘mouse’.
- 323<sub>7</sub> Replace ‘ $O(n^{-1/2})$ ’ by ‘ $O(n^{-1})$ ’.
- 323<sub>6</sub> Replace ‘1999’ by ‘2001’.
- 323<sub>3</sub> Replace ‘ $O(n^{-1})$ ’ by ‘ $O(n^{-2})$ ’.
- 325<sub>13</sub> = (14.5.2) This line should be
- $$f(\mathbf{x}; \boldsymbol{\lambda}, \kappa) = \{1 + \kappa(\boldsymbol{\lambda}^T \mathbf{x} + 1)\} \exp\{\kappa(\boldsymbol{\lambda}^T \mathbf{x} - 1)\}, \mathbf{x} \in S^2, |\boldsymbol{\lambda}| = 1, \quad (14.5.2)$$
- 325<sub>12</sub> Replace “and  $\boldsymbol{\lambda}$  is the ‘mean shape’” by
- “where  $\boldsymbol{\lambda}$  is the shape of  $(\boldsymbol{\mu}_1, \boldsymbol{\mu}_2, \boldsymbol{\mu}_3)$  and  $\kappa = \sum_{i=1}^3 (\boldsymbol{\mu}_i - \bar{\boldsymbol{\mu}})^2 / 4\sigma^2$ ”.
- 349<sub>6-5</sub> = (A.4) Replace  $\frac{(4p^2 - 1)(4p^2 - 9)}{2(8\kappa)^2}$  by  $\frac{(4p^2 - 1)(4p^2 - 9)}{2!(8\kappa)^2}$ .
- Replace  $\frac{(4p^2 - 1)(4p^2 - 9)(4p^2 - 25)}{2(8\kappa)^3}$   
by  $\frac{(4p^2 - 1)(4p^2 - 9)(4p^2 - 25)}{3!(8\kappa)^3}$ .
- 350<sup>10</sup> = (A.10) Replace the integral in the numerator by  $\int_{-1}^1 te^{\kappa t}(1 - t^2)^{(p-3)/2} dt$ .
- 398<sup>19</sup> Replace ‘reconstruction’ by ‘reconstructions’.
- 398<sub>14</sub> Insert ‘matrix’ before ‘Langevin’.
- 398<sub>13</sub> Replace ‘Matsuita’ by ‘Matsusita’.
- 398<sub>5</sub> Replace ‘likelihood’ by ‘likelihood’.
- 398<sub>2</sub> Replace ‘**53**’ by ‘**54**’.
- 402<sup>11</sup> Replace ‘1980’ by ‘1981’.
- 404<sup>26</sup> Replace ‘(1999)’ by ‘(2001)’.
- 404<sup>27</sup> Replace ‘*Submitted for publication.*’ by ‘*J. Multivariate Anal.*, **77**, 1–20.’.
- 406<sup>3</sup> Insert ‘matrix’ before ‘distribution’.
- 408<sub>16</sub> Replace ‘A-s 86’ by ‘AS 86’.

I am very grateful to all those who have pointed out errors in the text.

PEJ

21/2/14